iris/UnionLinkInst.v
@@ -151,10 +151,30 @@ Section union_link_inst.
     - iSplitR; [by iPureIntro |]. subst I. iExact "HE".
   Qed.
 
+  (* THE RECORD'S TAINT: the union's, or the era's WILD TOKEN (seccomp
+     design 10.5) -- which licenses its own era only, so THE RECORD'S PIN
+     NAMES THE ERA (10.7): every family arm but the taint already carries
+     [k = S gen_id] through [f0w] / [fhead] / [union_X] *)
+  Definition uT : iProp Σ := (UT ∨ usecc_tok ug (S gen_id))%I.
+  Global Instance uT_persistent : Persistent uT.
+  Proof using . rewrite /uT. apply _. Qed.
+  Global Instance uT_timeless : Timeless uT.
+  Proof using . rewrite /uT. apply _. Qed.
+
+  Definition upin (k : nat) (v : era_pins) : iProp Σ := (UPIN k v ∗ ⌜k = S gen_id⌝)%I.
+  Global Instance upin_persistent k v : Persistent (upin k v).
+  Proof using . rewrite /upin. apply _. Qed.
+  Global Instance upin_timeless k v : Timeless (upin k v).
+  Proof using . rewrite /upin. apply _. Qed.
+  Lemma upin_agree k v v' : upin k v -∗ upin k v' -∗ ⌜v = v'⌝.
+  Proof using .
+    iIntros "[H _] [H' _]". iApply (era_pin_agree (fgn_echo gf) with "H H'").
+  Qed.
+
   Definition union_params : gen_params U :=
     MkGP U ulmG_laws ulmG_hooks
-      UT _ _
-      UPIN _ _ (era_pin_agree (fgn_echo gf))
+      uT _ _
+      upin _ _ upin_agree
       (f0w gf) _ _
       uf0bwk _ _ (S gen_id) uf0w_bwk uf0w_bwk0 uf0bwk_agree
       (fhead gf) _ ufhead_cur ufhead_inp.
@@ -184,12 +204,60 @@ Section union_link_inst.
     iIntros "Hw". rewrite /f0w. iSplitR; [by iPureIntro | iExact "Hw"].
   Qed.
 
-  (* the links are the claim's: the bundle is the record equation *)
+  (* the links are the claim's: the bundle is the record equation.  THE
+     TAINT'S BYTE is the union's taint or the wild token's licence at the
+     pin's era; THE BLOCK-FIRST BYTE's escape at the [seccomp x] line is
+     the token, which is the record's taint (the writer's witness puts it
+     at the era's number) *)
   Lemma union_links_gl : union_links ug -∗ glinks U union_params.
   Proof using .
     iIntros "Hlk". iDestruct (union_links_eq with "Hlk") as %Hc.
-    iApply (peclV_glinks pg U (ucparams ug) (ulm_byte_laws adm_u_g adm_s_off) ∅ (uwa ug) Hc
-              union_params eq_refl eq_refl uf0w_cw (or_introl I) ufhead_boot).
+    rewrite /glinks /gl_w /gl_blk /gl_pro /gl_head /gl_taint.
+    cbn [gT gPIN gW gH union_params].
+    iSplitR; [| iSplitR; [| iSplitR; [| iSplitR]]].
+    - iIntros "!>" (k v P0 b ps0 cs0 s0 I0 Φ)
+        "%H1 %H2 %H3 [#Hpin _] #Hw Ht #Hps #Hcs #HE HΦ".
+      iApply (union_write_link ug Hc k v P0 b ps0 cs0 s0 I0 Φ H1 H2 H3
+                with "Hpin Ht Hps Hcs HE [Hw] [HΦ]"); [by iApply uf0w_cw |].
+      iIntros "[(Ht & Hps' & Hcs' & HE' & _) | #HT]"; iApply "HΦ";
+        [iLeft; by iFrame "Ht Hps' Hcs' HE'" | iRight; by iLeft].
+    - iIntros "!>" (k v P0 a b ps0 cs0 s0 I0 Φ)
+        "%H1 %H2 %H3 %H4 %H5 %H6 %H7 %H8 [#Hpin %Hk] #Hw Ht #Hps #Hcs #HE HΦ".
+      rewrite /lm_abs /lm_line_at in H6 H8.
+      iApply (union_write_link_blk ug Hc k v P0 a b ps0 cs0 s0 I0 Φ H1 H2 H3 H4 H5 H6 H7 H8
+                with "Hpin Ht Hps Hcs HE [Hw] [HΦ]"); [by iApply uf0w_cw |].
+      iIntros "[[(Ht & Hps' & Hcs' & HE' & _) | #HT] | (#Htok & _ & _)]"; iApply "HΦ";
+        [iLeft; by iFrame "Ht Hps' Hcs' HE'" | iRight; by iLeft |].
+      iRight. iRight. subst k. iExact "Htok".
+    - iIntros "!>" (k v P0 a b ps0 cs0 s0 I0 Φ)
+        "%H1 %H2 %H3 %H4 %H5 %H6 %H7 %H8 [#Hpin _] #Hw Ht #Hps #Hcs #HE HΦ".
+      iApply (union_write_link_pro ug Hc k v P0 a b ps0 cs0 s0 I0 Φ
+                H1 H2 H3 H4 H5 H6 H7 H8
+                with "Hpin Ht Hps Hcs HE [Hw] [HΦ]"); [by iApply uf0w_cw |].
+      iIntros "[(Ht & Hps' & Hcs' & HE' & _) | #HT]"; iApply "HΦ";
+        [iLeft; by iFrame "Ht Hps' Hcs' HE'" | iRight; by iLeft].
+    - iIntros "!>" (k v I a b Φ) "%H1 %H2 [#Hpin _] Hh HΦ".
+      iDestruct (ufhead_boot with "Hh") as "(Ht & #Hps & #Hcs & #HE & %s0 & %Hok & Hbt & Hwb)".
+      iApply (union_write_link_first ug Hc k v a b s0 Φ Hok H1 H2
+                with "Hpin Ht Hps Hcs HE Hbt [HΦ Hwb]").
+      iIntros "[(Ht & Hps' & Hcs' & HE' & Hw) | #HT]"; iApply "HΦ"; [| iRight; by iLeft].
+      iLeft. iExists s0. iFrame "Ht Hps' Hcs' HE'". by iApply "Hwb".
+    - iIntros "!>" (k v b Φ) "[_ %Hk] #HT HΦ". rewrite /uT.
+      iDestruct "HT" as "[#HU | #Htok]".
+      + iApply (union_write_link_taint ug Hc with "HU"). iIntros "_". iApply "HΦ". by iLeft.
+      + subst k. iApply (union_write_link_wild ug Hc with "Htok"). iApply "HΦ". by iRight.
+  Qed.
+
+  (* the taint's byte at the era's own number, for a device at it *)
+  Lemma union_links_gl_taint_now :
+    union_links ug -∗ gl_taint_at U union_params (S gen_id).
+  Proof using .
+    iIntros "Hlk". iDestruct (union_links_eq with "Hlk") as %Hc.
+    rewrite /gl_taint_at. cbn [gT union_params].
+    iIntros "!>" (b Φ) "#HT HΦ". rewrite /uT.
+    iDestruct "HT" as "[#HU | #Htok]".
+    - iApply (union_write_link_taint ug Hc with "HU"). iIntros "_". iApply "HΦ". by iLeft.
+    - iApply (union_write_link_wild ug Hc with "Htok"). iApply "HΦ". by iRight.
   Qed.
 
   (* =================================================================== *)
@@ -199,15 +267,15 @@ Section union_link_inst.
       (ws : list (list mobs * bv 8)) :
     (0 < length ws)%nat ->
     uread_ret ug k v n ws -∗
-    UT ∨ (∃ (ps0 cs0 : list nat) (s0 : fstate) (J : list (bv 8)),
+    uT ∨ (∃ (ps0 cs0 : list nat) (s0 : fstate) (J : list (bv 8)),
             ⌜length J = (n + length ws)%nat⌝ ∗ ⌜lm_rd_stage U ps0 cs0 s0 J⌝
             ∗ inp_lb v J ∗ turn_lb v (length (lm_proc_before U ps0 cs0 s0 J))
             ∗ ps_lb v ps0 ∗ cs_lb v cs0 ∗ uf0bwk k s0).
   Proof using .
-    intros Hws. iIntros "Hr". rewrite /uread_ret /vread_ret.
-    iDestruct "Hr" as "[[#HT _] | [_ Hfacts]]"; [by iLeft |].
+    intros Hws. iIntros "Hr". rewrite /uread_ret.
+    iDestruct "Hr" as "[[#HT _] | [_ Hfacts]]"; [iLeft; by iLeft |].
     iDestruct "Hfacts" as (pops dl)
-      "(%Hrok & %Hdl & %Hpref & %Hidx & %Hdsc & %Hboots & #Hinp & %Hdi & Hrest)".
+      "(%Hrok & %Hdl & %Hpref & %Hidx & %Hdsc & %Hboots & #Hinp & %Hdi & Hrest & _)".
     iDestruct "Hrest" as "[%Hws0 | Hbb]".
     { exfalso. rewrite Hws0 in Hws. cbn in Hws. lia. }
     iDestruct "Hbb" as (cs0 ps0 s0) "(#Hcs0 & #Hps0 & #Hw & %Hbd & #Htlb & %Hrs)".
@@ -221,14 +289,14 @@ Section union_link_inst.
 
   Lemma uturn0 (k : nat) :
     fturn_pre gf k -∗
-    (∃ v : era_pins, UPIN k v ∗ dl_cnt v (1/2) 0%nat ∗ inp_lb v [])
-    ∗ (∃ v : era_pins, UPIN k v ∗ gwc_ban U union_params k v [] 0%nat).
+    (∃ v : era_pins, upin k v ∗ dl_cnt v (1/2) 0%nat ∗ inp_lb v [])
+    ∗ (∃ v : era_pins, upin k v ∗ gwc_ban U union_params k v [] 0%nat).
   Proof using .
     rewrite /fturn_pre /FileOut.fturn_core.
     iIntros "(%Hk & Ht & Hpre)".
     iDestruct "Ht" as (v vf) "(#Hpin & #Hvf & Htn & Hdl & #Hcs & #Hps & #HE)".
-    iSplitL "Hdl"; [iExists v; by iFrame "Hpin Hdl HE" |].
-    iExists v. iFrame "Hpin". rewrite /gwc_ban. iRight. iLeft.
+    iSplitL "Hdl"; [iExists v; iFrame "Hpin Hdl HE"; by iPureIntro |].
+    iExists v. iSplitR; [iFrame "Hpin"; by iPureIntro |]. rewrite /gwc_ban. iRight. iLeft.
     iSplitR; [by iPureIntro |]. rewrite /gH /union_params /fhead.
     iSplitR; [by iPureIntro |]. iSplitR; [by iPureIntro |].
     iFrame "Htn Hps Hcs HE Hpre". iExists vf. iExact "Hvf".
@@ -274,16 +342,16 @@ Section union_link_inst.
   Lemma union_X_dollar (k : nat) (v : era_pins) (I : list (bv 8)) (b : bv 8)
       (Φ : iProp Σ) :
     b = u_prompt !!! 0%nat ->
-    UPIN k v -∗ union_links ug -∗ union_X k v I -∗
+    upin k v -∗ union_links ug -∗ union_X k v I -∗
     (gwc_sp_t U union_params k v I -∗ Φ) -∗ out_link Uart0 k b Φ.
   Proof using .
-    intros Hb. iIntros "#Hpin #Hlk Hx HΦ".
+    intros Hb. iIntros "[#Hpin _] #Hlk Hx HΦ".
     iDestruct (union_links_eq with "Hlk") as %Hc.
     iDestruct "Hx" as "[%Hk Hx]".
     iDestruct "Hx" as (sR lR pre) "([%HlR [%Ha %Hbl]] & Hpw)".
     iApply (union_file_link ug Hc k v I sR lR pre b Φ HlR Ha Hbl Hb with "Hpw").
     iIntros "Hret". iApply "HΦ". rewrite /gwc_sp_t.
-    iDestruct "Hret" as "[Hx | #HT]"; [| by iRight].
+    iDestruct "Hret" as "[Hx | #HT]"; [| iRight; by iLeft].
     iDestruct "Hx" as (ps cs s0 P) "([%Hw %Htie] & #HW & Htn & Hps & Hcs & HE)".
     iLeft. iExists ps, (cs ++ [pv_enc pview_unionU lR (PLRun pre)]), s0,
       (P + S (length pre))%nat.
@@ -307,9 +375,9 @@ Section union_link_inst.
       uturn0 urresw urresw_persistent urresw_timeless urresw_res
       (ualt_code (UR RFSilent)).
 
-  Lemma union_inst_T : lk_T union_link_inst = UT.
+  Lemma union_inst_T : lk_T union_link_inst = uT.
   Proof using . reflexivity. Qed.
-  Lemma union_inst_pin : lk_pin union_link_inst = UPIN.
+  Lemma union_inst_pin : lk_pin union_link_inst = upin.
   Proof using . reflexivity. Qed.
   Lemma union_inst_links : lk_links union_link_inst = union_links ug.
   Proof using . reflexivity. Qed.
