iris/UnionReadInst.v
@@ -87,22 +87,25 @@ Section union_read_inst.
 
   Local Lemma uri_rd (k n : nat) (v : era_pins)
       (ws : list (list mobs * bv 8)) (Φ : iProp Σ) :
-    ⊢ union_links ug -∗ UPIN k v -∗ dl_cnt v (1/2) n -∗
+    ⊢ union_links ug -∗ upin ug k v -∗ dl_cnt v (1/2) n -∗
       (uread_ret ug k v n ws -∗ Φ) -∗
       cons_link Uart0 k (ConsLog.EvRead ws) Φ.
   Proof using .
-    iIntros "#Hlk #Hpin Hdl HΦ".
+    iIntros "#Hlk [#Hpin _] Hdl HΦ".
     iDestruct (union_links_rd with "Hlk") as "#Hrdl".
     iApply ("Hrdl" $! k v n ws with "Hpin Hdl HΦ").
   Qed.
 
-  Local Lemma uri_rd_taint (k : nat) (ws : list (list mobs * bv 8)) (Φ : iProp Σ) :
-    ⊢ union_links ug -∗ UT -∗ (UT -∗ Φ) -∗
-      cons_link Uart0 k (ConsLog.EvRead ws) Φ.
+  Local Lemma uri_rd_taint (ws : list (list mobs * bv 8)) (Φ : iProp Σ) :
+    ⊢ union_links ug -∗ uT ug -∗ (uT ug -∗ Φ) -∗
+      cons_link Uart0 (S gen_id) (ConsLog.EvRead ws) Φ.
   Proof using .
-    iIntros "#Hlk HT HΦ".
-    iDestruct (union_links_rd_taint with "Hlk") as "#Hrdt".
-    iApply ("Hrdt" $! k ws with "HT HΦ").
+    iIntros "#Hlk #HT HΦ". rewrite /uT.
+    iDestruct "HT" as "[#HU | #Htok]".
+    - iDestruct (union_links_rd_taint with "Hlk") as "#Hrdt".
+      iApply ("Hrdt" $! (S gen_id) ws with "HU [HΦ]"). iIntros "_". iApply "HΦ". by iLeft.
+    - iDestruct (union_links_eq with "Hlk") as %Hc.
+      iApply (union_read_link_wild ug Hc with "Htok"). iApply "HΦ". by iRight.
   Qed.
 
   (* THE LAST CONSUMED ENTRY'S TAG ([FileReadInst]'s, verbatim): the
@@ -162,7 +165,7 @@ Section union_read_inst.
     cons_window sl (length I) dd g0 hs ->
     sl `prefix_of` sl' ->
     (forall j : nat, (j < dc)%nat -> ws !! j = sl' !! (length I + j)%nat) ->
-    ⊢ UPIN (S gen_id) v -∗ inp_lb v I -∗
+    ⊢ upin ug (S gen_id) v -∗ inp_lb v I -∗
       urresw ug v I -∗
       uread_ret ug (S gen_id) v (length I) ws -∗
       ([∗ list] hh ∈ hs, riscv_rx_tag hh) -∗
@@ -173,14 +176,19 @@ Section union_read_inst.
            ⌜length J = dc⌝ ∗ ⌜lm_disc_input U (I ++ J)⌝
            ∗ ⌜(0 < dd)%nat -> g0 0%nat = J !!! 0%nat⌝
            ∗ inp_lb v (I ++ J) ∗ urresw ug v (I ++ J))
-      ∨ UT.
+      ∨ uT ug.
   Proof using Htag.
     intros Hddc Hlws Hwinf Hpre2 Hwsj.
-    iIntros "#Hpin #HE0 [#Hres0 #Hw0] Hret #Htags #Hsw #Hlb2".
-    rewrite /uread_ret /vread_ret.
-    iDestruct "Hret" as "[[#HT _] | [Hdlr Hfacts]]"; [ by iRight | ].
+    iIntros "[#Hpin _] #HE0 [#Hres0 #Hw0] Hret #Htags #Hsw #Hlb2".
+    rewrite /uread_ret.
+    iDestruct "Hret" as "[[#HT _] | [Hdlr Hfacts]]"; [ iRight; by iLeft | ].
     iDestruct "Hfacts" as (pops dl)
-      "(%Hrok & %Hdl & %Hpref & %Hidx & %Hdsce & %Hboots & #HEin & %Hdinp & Hrest)".
+      "(%Hrok & %Hdl & %Hpref & %Hidx & %Hdsce & %Hboots & #HEin & %Hdinp & Hrest & Htok)".
+    (* A READ THAT COMPLETES THE [seccomp x] LINE: the era is wild, and the
+       reader leaves with the token (seccomp design 10.4) *)
+    destruct (decide (uread_wild (snd <$> (dl ++ ws)) ws)) as [Hwd | _].
+    { iDestruct ("Htok" with "[//]") as "#Htk". iRight. rewrite /uT.
+      iDestruct "Htk" as "[Htk | HU]"; [by iRight | by iLeft]. }
     iEval (rewrite Hlws) in "Hdlr".
     iDestruct (inp_lb_cmp v I (snd <$> (dl ++ ws)) with "HE0 HEin") as %Hcmp.
     assert (Hlen' : length (snd <$> (dl ++ ws)) = (length I + dc)%nat).
@@ -241,7 +249,7 @@ Section union_read_inst.
       - rewrite last_app Hlast. reflexivity.
       - exact Hsh.
       - exact Hw. }
-    iDestruct "Hwn" as "[#Hwn | #HT]"; [ | by iRight ].
+    iDestruct "Hwn" as "[#Hwn | #HT]"; [ | iRight; by iLeft ].
     iLeft. iFrame "Hdlr". iExists J.
     iSplitR; [ by iPureIntro | ]. iSplitR; [ by iPureIntro | ].
     iSplitR; [ | iFrame "HEn"; rewrite /urresw; iFrame "Hresn Hwn" ].
